---
title: "MATH4428 Lecture 11: Lagrange Multiplies"
date: 2020-02-14
math: true 
categories: [MATH4428]
---

## Announcements

Homework is due next Wednesday.

## Lecture

(labeling sections often proves too difficult)

### Linear Transformation

A space, $S$, is linear if $\forall x,y\in S x+y\in S$ and $\forall x\in S, c\in \mathbb{R}, cx\in S$.

If, for some $n\times n$ matrix $A$, $\forall x\in\mathbb{R}^n\to y=Ax$ then the transformation $x\to y$ is linear. 

Given $A^T=A$, $(Ax,y)=(x,Ay)$.

(I'm currently confused by the notation, he's drawn a circle and what appear to be points, but it seems we are just calculating maximal eigenvalues?)

### Multivariable Chain Rule

$$\dfrac{d}{dt}f\left(x(t),y(t)\right)= f_x\cdot\dfrac{dx}{dt}+f_y\cdot\dfrac{dy}{dt}$$

Safonov claims $\Nabla A(x,x)=2Ax$ which confirms the suspicion that things are *definitely* being overcomplicated. ($\nabla$ is the differential operator, del.)

I've just realized that his parenthetical notation is a dot product! Everything now makes sense, except for why he would use that notation.

### "Practical" Application

*Given $A^m$, what is $A^{1/m}$?* 

If $\lambda_j>0$, then $A=\sum \lambda_j v_j v_j^T\implies A^{1/m} = \sum \lambda_j^{1/m} v_j v_j^T$.

**Pf:** Let $B^m=A$ for $m=2$. Then, $$BB=\sum_j \lamda_j^{1/2} v_j v_j^T\cdot\sum_k \lambda_k^{1/2} v_k v_k^T.$$

That can be rewritten as 

$$\sum_{j,k} \lambda_j^{1/2} \lambda_k^{1/2} \underbrace{v_j(v_j^T v_k)v_k^T}_{\delta_{jk}} = \sum_j \lambda_j v_j v_j^T.$$

(I need a ton of vector hats, I keep forgetting because Safonov does not use them.)

### Lagrange Multipliers

(writing this out with his notation so I can match it better in the future)

To find the max of $f(x)$, equal to $S=\{g=C\}$ (new notation, I suspect that is his constraint) we can use the gradient $\delta f$. We know $\nabla f \perp \{ f=c, c\in\mathbb{R} \}$. (That just means that the gradient is perpendicular to any level set.) Solve $\nabla f =\lambda \nabla g$.

He instead wrote $F(x,\lambda) = f(x)-\lambda g(x)$ subject to $\nabla_x F=\nabla f - \lambda\nabla g =0, S=\{g=0\}\implies \dfrac{d}{d\lambda} F = -g=0$. That does not yet make sense to me.

#### Cylinder Example

$f(r,h)=\pi r^2h$ and $S=2\pi r(r+h)$.

Then, $$\nabla f = \lambda\nabla g\implies \begin{bmatrix}2rh\\r^2\end{bmatrix}=2\lambda\begin{bmatrix}2r+h\\r\end{bmatrix}.$$

This tells us that $r^2=2\lambda r \\implies r=2\lambda$. Plugging that into the earlier equation, $h=4\lambda$.